natmap.v
@@ -1,0 +1,230 @@
+(* Copyright (c) 2012-2013, Robbert Krebbers. *)
+(* This file is distributed under the terms of the BSD license. *)
+(** This files implements finite maps whose keys range over Coq's data type of
+unary natural numbers [nat]. *)
+Require Import fin_maps.
+
+Notation natmap_raw A := (list (option A)).
+Definition natmap_wf {A} (l : natmap_raw A) :=
+  match last l with
+  | None => True
+  | Some x => is_Some x
+  end.
+Instance natmap_wf_pi {A} (l : natmap_raw A) : ProofIrrel (natmap_wf l).
+Proof. unfold natmap_wf. case_match; apply _. Qed.
+
+Lemma natmap_wf_inv {A} (o : option A) (l : natmap_raw A)  :
+  natmap_wf (o :: l) → natmap_wf l.
+Proof. by destruct l. Qed.
+Lemma natmap_wf_lookup {A} (l : natmap_raw A) :
+  natmap_wf l → l ≠ [] → ∃ i x, mjoin (l !! i) = Some x.
+Proof.
+  intros Hwf Hl. induction l as [|[x|] l IH]; simpl.
+  * done.
+  * exists 0. simpl. eauto.
+  * destruct IH as (i&x&?); eauto using natmap_wf_inv.
+    { intro. subst. inversion Hwf. }
+    by exists (S i) x.
+Qed.
+
+Definition natmap (A : Type) : Type := sig (@natmap_wf A).
+
+Instance natmap_empty {A} : Empty (natmap A) := [] ↾ I.
+Instance natmap_lookup {A} : Lookup nat A (natmap A) :=
+  λ i m, mjoin (`m !! i).
+
+Fixpoint natmap_singleton_raw {A} (i : nat) (x : A) : natmap_raw A :=
+  match i with
+  | 0 => [Some x]
+  | S i => None :: natmap_singleton_raw i x
+  end.
+Lemma natmap_singleton_wf {A} (i : nat) (x : A) :
+  natmap_wf (natmap_singleton_raw i x).
+Proof.
+  unfold natmap_wf, last.
+  induction i as [|i]; simpl; repeat case_match; simplify_equality; eauto.
+  by destruct i.
+Qed.
+Lemma natmap_lookup_singleton_raw {A} (i : nat) (x : A) :
+  mjoin (natmap_singleton_raw i x !! i) = Some x.
+Proof. induction i; simpl; auto. Qed.
+Lemma natmap_lookup_singleton_raw_ne {A} (i j : nat) (x : A) :
+  i ≠ j → mjoin (natmap_singleton_raw i x !! j) = None.
+Proof. revert j; induction i; intros [|?]; simpl; auto with congruence. Qed.
+Hint Rewrite @natmap_lookup_singleton_raw : natmap.
+
+Definition natmap_cons_canon {A} (o : option A) (l : natmap_raw A) :=
+  match o, l with
+  | None, [] => []
+  | _, _ => o :: l
+  end.
+Lemma natmap_cons_canon_wf {A} (o : option A) (l : natmap_raw A) :
+  natmap_wf l → natmap_wf (natmap_cons_canon o l).
+Proof. unfold natmap_wf, last. destruct o, l; simpl; eauto. Qed.
+Lemma natmap_cons_canon_O {A} (o : option A) (l : natmap_raw A) :
+  mjoin (natmap_cons_canon o l !! 0) = o.
+Proof. by destruct o, l. Qed.
+Lemma natmap_cons_canon_S {A} (o : option A) (l : natmap_raw A) i :
+  natmap_cons_canon o l !! S i = l !! i.
+Proof. by destruct o, l. Qed.
+Hint Rewrite @natmap_cons_canon_O @natmap_cons_canon_S : natmap.
+
+Definition natmap_alter_raw {A} (f : option A → option A) :
+    nat → natmap_raw A → natmap_raw A :=
+  fix go i l {struct l} :=
+  match l with
+  | [] =>
+     match f None with
+     | Some x => natmap_singleton_raw i x
+     | None => []
+     end
+  | o :: l =>
+     match i with
+     | 0 => natmap_cons_canon (f o) l
+     | S i => natmap_cons_canon o (go i l)
+     end
+  end.
+Lemma natmap_alter_wf {A} (f : option A → option A) i l :
+  natmap_wf l → natmap_wf (natmap_alter_raw f i l).
+Proof.
+  revert i. induction l; [intro | intros [|?]]; simpl; repeat case_match;
+    eauto using natmap_singleton_wf, natmap_cons_canon_wf, natmap_wf_inv.
+Qed.
+Instance natmap_alter {A} : PartialAlter nat A (natmap A) := λ f i m,
+  natmap_alter_raw f i (`m)↾natmap_alter_wf _ _ _ (proj2_sig m).
+Lemma natmap_lookup_alter_raw {A} (f : option A → option A) i l :
+  mjoin (natmap_alter_raw f i l !! i) = f (mjoin (l !! i)).
+Proof.
+  revert i. induction l; intros [|?]; simpl; repeat case_match; simpl;
+    autorewrite with natmap; auto.
+Qed.
+Lemma natmap_lookup_alter_raw_ne {A} (f : option A → option A) i j l :
+  i ≠ j → mjoin (natmap_alter_raw f i l !! j) = mjoin (l !! j).
+Proof.
+  revert i j. induction l; intros [|?] [|?] ?; simpl;
+    repeat case_match; simpl; autorewrite with natmap; auto with congruence.
+  rewrite natmap_lookup_singleton_raw_ne; congruence.
+Qed.
+
+Definition natmap_merge_aux {A B} (f : option A → option B) :
+    natmap_raw A → natmap_raw B :=
+  fix go l :=
+  match l with
+  | [] => []
+  | o :: l => natmap_cons_canon (f o) (go l)
+  end.
+Lemma natmap_merge_aux_wf {A B} (f : option A → option B) l :
+  natmap_wf l → natmap_wf (natmap_merge_aux f l).
+Proof. induction l; simpl; eauto using natmap_cons_canon_wf, natmap_wf_inv. Qed.
+Lemma natmap_lookup_merge_aux {A B} (f : option A → option B) l i :
+  f None = None →
+  mjoin (natmap_merge_aux f l !! i) = f (mjoin (l !! i)).
+Proof.
+  revert i. induction l; intros [|?]; simpl; autorewrite with natmap; auto.
+Qed.
+Hint Rewrite @natmap_lookup_merge_aux : natmap.
+
+Definition natmap_merge_raw {A B C} (f : option A → option B → option C) :
+    natmap_raw A → natmap_raw B → natmap_raw C :=
+  fix go l1 l2 :=
+  match l1, l2 with
+  | [], l2 => natmap_merge_aux (f None) l2
+  | l1, [] => natmap_merge_aux (flip f None) l1
+  | o1 :: l1, o2 :: l2 => natmap_cons_canon (f o1 o2) (go l1 l2)
+  end.
+Lemma natmap_merge_wf {A B C} (f : option A → option B → option C) l1 l2 :
+  natmap_wf l1 → natmap_wf l2 → natmap_wf (natmap_merge_raw f l1 l2).
+Proof.
+  revert l2. induction l1; intros [|??]; simpl;
+    eauto using natmap_merge_aux_wf, natmap_cons_canon_wf, natmap_wf_inv.
+Qed.
+Lemma natmap_lookup_merge_raw {A B C} (f : option A → option B → option C) l1 l2 i :
+  f None None = None →
+  mjoin (natmap_merge_raw f l1 l2 !! i) = f (mjoin (l1 !! i)) (mjoin (l2 !! i)).
+Proof.
+  intros. revert i l2. induction l1; intros [|?] [|??]; simpl;
+    autorewrite with natmap; auto.
+Qed.
+Instance natmap_merge: Merge natmap := λ A B C f m1 m2,
+  natmap_merge_raw f _ _ ↾ natmap_merge_wf _ _ _ (proj2_sig m1) (proj2_sig m2).
+
+Fixpoint natmap_to_list_raw {A} (i : nat) (l : natmap_raw A) : list (nat * A) :=
+  match l with
+  | [] => []
+  | None :: l => natmap_to_list_raw (S i) l
+  | Some x :: l => (i,x) :: natmap_to_list_raw (S i) l
+  end.
+Lemma natmap_elem_of_to_list_raw_aux {A} j (l : natmap_raw A) i x :
+  (i,x) ∈ natmap_to_list_raw j l ↔ ∃ i', i = i' + j ∧ mjoin (l !! i') = Some x.
+Proof.
+  split.
+  * revert j. induction l as [|[y|] l IH]; intros j; simpl.
+    + by rewrite elem_of_nil.
+    + rewrite elem_of_cons. intros [?|?]; simplify_equality.
+      - by exists 0.
+      - destruct (IH (S j)) as (i'&?&?); auto.
+        exists (S i'); simpl; auto with lia.
+    + intros. destruct (IH (S j)) as (i'&?&?); auto.
+      exists (S i'); simpl; auto with lia.
+  * intros (i'&?&Hi'). subst. revert i' j Hi'.
+    induction l as [|[y|] l IH]; intros i j ?; simpl.
+    + done.
+    + destruct i as [|i]; simplify_equality; [left|].
+      right. rewrite NPeano.Nat.add_succ_comm. by apply (IH i (S j)).
+    + destruct i as [|i]; simplify_equality.
+      rewrite NPeano.Nat.add_succ_comm. by apply (IH i (S j)).
+Qed.
+Lemma natmap_elem_of_to_list_raw {A} (l : natmap_raw A) i x :
+  (i,x) ∈ natmap_to_list_raw 0 l ↔ mjoin (l !! i) = Some x.
+Proof.
+  rewrite natmap_elem_of_to_list_raw_aux. setoid_rewrite plus_0_r. naive_solver.
+Qed.
+Lemma natmap_to_list_raw_nodup {A} i (l : natmap_raw A) :
+  NoDup (natmap_to_list_raw i l).
+Proof.
+  revert i. induction l as [|[?|] ? IH]; simpl; try constructor; auto.
+  rewrite natmap_elem_of_to_list_raw_aux. intros (?&?&?). lia.
+Qed.
+Instance natmap_to_list {A} : FinMapToList nat A (natmap A) := λ m,
+  natmap_to_list_raw 0 (`m).
+
+Definition natmap_map_raw {A B} (f : A → B) : natmap_raw A → natmap_raw B :=
+  fmap (fmap f).
+Lemma natmap_map_wf {A B} (f : A → B) l :
+  natmap_wf l → natmap_wf (natmap_map_raw f l).
+Proof.
+  unfold natmap_wf, last.
+  induction l; simpl; repeat case_match; simplify_equality; eauto.
+  simpl. by rewrite fmap_is_Some.
+Qed.
+Lemma natmap_lookup_map_raw {A B} (f : A → B) i l :
+  mjoin (natmap_map_raw f l !! i) = f <$> mjoin (l !! i).
+Proof. unfold natmap_map_raw. rewrite list_lookup_fmap. by destruct (l !! i). Qed.
+Instance natmap_map: FMap natmap := λ A B f m,
+  natmap_map_raw f _ ↾ natmap_map_wf _ _ (proj2_sig m).
+
+Instance: FinMap nat natmap.
+Proof.
+  split.
+  * unfold lookup, natmap_lookup. intros A [l1 Hl1] [l2 Hl2] E.
+    apply (sig_eq_pi _). revert l2 Hl1 Hl2 E. simpl.
+    induction l1 as [|[x|] l1 IH]; intros [|[y|] l2] Hl1 Hl2 E; simpl in *.
+    + done.
+    + by specialize (E 0).
+    + destruct (natmap_wf_lookup (None :: l2)) as [i [??]]; auto with congruence.
+    + by specialize (E 0).
+    + f_equal. apply (E 0). apply IH; eauto using natmap_wf_inv.
+      intros i. apply (E (S i)).
+    + by specialize (E 0).
+    + destruct (natmap_wf_lookup (None :: l1)) as [i [??]]; auto with congruence.
+    + by specialize (E 0).
+    + f_equal. apply IH; eauto using natmap_wf_inv.
+      intros i. apply (E (S i)).
+  * done.
+  * intros ?? [??] ?. apply natmap_lookup_alter_raw.
+  * intros ?? [??] ??. apply natmap_lookup_alter_raw_ne.
+  * intros ??? [??] ?. apply natmap_lookup_map_raw.
+  * intros ? [??]. by apply natmap_to_list_raw_nodup.
+  * intros ? [??] ??. by apply natmap_elem_of_to_list_raw.
+  * intros ????? [??] [??] ?. by apply natmap_lookup_merge_raw.
+Qed.
